lemmas about probWhileSplit

SampCert/DifferentialPrivacy/Queries/UnboundedMax/Properties.lean
@@ -28,10 +28,136 @@ noncomputable section
 namespace SLang
 
 /--
-Probability that privMax evaluates to k, ie, the probability
-the the loop unrolls exactly k times.
+``SLang`` value obtained by applying a loop body exactly ``n`` times to a given distribution
 -/
-def privMax_cut (ε₁ ε₂ : ℕ+) (l : List ℕ) (N : ℕ) : SLang ℤ := do
+def probWhileSplit (cond : T → Bool) (body : T → SLang T) (continuation : T -> SLang T) (n : Nat) (a : T) : SLang T :=
+  match n with
+  | Nat.zero => continuation a
+  | Nat.succ n => do
+    if cond a
+      then
+        let v ← body a
+        probWhileSplit cond body continuation n v
+      else
+        return a
+
+    -- probWhileFunctional cond body (probWhileSplit cond body base n) a
+
+/--
+probWhileCut is probWhileSplit applied to the zero distribution
+-/
+lemma probWhileCut_probWhileSplit_zero (cond : T → Bool) (body : T → SLang T) (n : Nat) :
+    probWhileCut cond body n = probWhileSplit cond body (fun _ => probZero) n := by
+  apply funext
+  induction n
+  · simp [probWhileCut, probWhileSplit]
+  · rename_i n IH
+    simp [probWhileCut, probWhileSplit]
+    rw [funext IH]
+    intro _
+    rfl
+
+/--
+Evaluate probWhileSplit when out of steps
+-/
+lemma probWhileSplit_zero (cond : T → Bool) (body : T → SLang T) (continuation : T -> SLang T) (init : T):
+    probWhileSplit cond body continuation 0 init = continuation init := by
+  simp [probWhileSplit]
+
+/--
+probWhileSplit is constant when the condition is false
+-/
+lemma probWhileSplit_cond_false_cst (cond : T → Bool) (body : T → SLang T) (continuation : T -> SLang T)
+    (n : Nat) (init : T) (HF : cond init ≠ true) :
+    probWhileSplit cond body continuation (Nat.succ n) init =
+    probPure init := by
+  rw [probWhileSplit]
+  split
+  · exfalso
+    simp_all
+  rfl
+
+/--
+Move an iterate of of probWhileSplit into the continuation.
+-/
+lemma probWhileSplit_succ_l (cond : T → Bool) (body : T → SLang T) (continuation : T -> SLang T) (n : Nat) (init : T):
+    probWhileSplit cond body continuation (Nat.succ n) init =
+    (probWhileSplit cond body (probWhileSplit cond body continuation n) 1 init) := by
+  apply funext
+  intro _
+  simp [probWhileSplit]
+
+/--
+Move multiple iterates of of probWhileSplit into the continuation.
+-/
+lemma probWhileSplit_add_l (cond : T → Bool) (body : T → SLang T) (continuation : T -> SLang T) (m n : Nat) (init : T):
+    probWhileSplit cond body continuation (n + m) init =
+    (probWhileSplit cond body (probWhileSplit cond body continuation n) m init) := by
+  revert init
+  induction m
+  · intro init
+    rw [probWhileSplit_zero]
+    simp only [add_zero]
+  · intro init
+    rename_i m' IH
+    rw [probWhileSplit_succ_l]
+    rw [<- (funext IH)]
+    rw [<- probWhileSplit_succ_l]
+    rfl
+
+
+/--
+Move iterates of probWhileSplit into the initial value, when the continuation is probPure
+
+Probably no use for this theorem
+-/
+lemma probWhileSplit_succ_r (cond : T → Bool) (body : T → SLang T) (n : Nat) (init : T):
+    probWhileSplit cond body probPure (Nat.succ n) init =
+    (probWhileSplit cond body probPure 1 init)  >>=  (probWhileSplit cond body probPure n) := by
+  apply funext
+  intro x
+  have H : (probWhileSplit cond body probPure 1 init) = if (cond init) then (body init) >>= probPure else pure init := by
+    apply funext
+    intro x
+    rw [probWhileSplit]
+    split
+    · simp [probWhileSplit]
+    · rfl
+  rw [H]
+  simp only [probWhileSplit]
+  split
+  · simp
+  · have H : (pure init >>= probWhileSplit cond body probPure n) = pure init := by
+      apply funext
+      intro x
+      simp [pure_apply]
+      conv =>
+        lhs
+        enter [1, a]
+      rw [ENNReal.tsum_eq_add_tsum_ite init]
+      simp
+      cases n
+      · simp [probWhileSplit]
+        rw [ENNReal.tsum_eq_zero.mpr ?G1]
+        case G1 =>
+          intro i
+          split <;> rfl
+        simp
+      · rename_i n'
+        rw [probWhileSplit_cond_false_cst _ _ _ _ _ (by trivial)]
+        simp [probPure]
+        rw [ENNReal.tsum_eq_zero.mpr ?G1]
+        case G1 =>
+          intro i
+          split <;> rfl
+        simp
+    rw [H]
+
+
+/--
+privMax unrolled at most k times
+-/
+def privMax_cut (ε₁ ε₂ : ℕ+) (l : List ℕ) (N : ℕ) : SLang ℕ := do
   let τ <- privNoiseZero ε₁ (2 * ε₂)
   let (k, _) <-
     (probWhileCut
@@ -43,6 +169,68 @@ def privMax_cut (ε₁ ε₂ : ℕ+) (l : List ℕ) (N : ℕ) : SLang ℤ := do
       N
       ((0 : ℕ), <- privNoiseZero ε₁ (4 * ε₂)))
   return k
+
+
+-- lemma privMax_cut_zero (ε₁ ε₂ : ℕ+) (l : List ℕ) (v : ℤ) :
+--     privMax_cut ε₁ ε₂ l 0 v = 0 := by
+--   simp [privMax_cut]
+--   aesop
+
+/--
+Threshold (in terms of N and v) for the support of privMax_cut, namely, N = v
+-/
+lemma privMax_cut_boundary (ε₁ ε₂ : ℕ+) (l : List ℕ) (N : ℕ) :
+    privMax_cut ε₁ ε₂ l N N = 0 := by
+  simp [privMax_cut]
+  intro τ
+  right
+  intro v0
+  right
+  intro r vr Hr
+  subst Hr
+  induction N
+  · aesop
+  · rename_i n' IH
+    -- rw [probWhileCut_unfold_1]
+    -- simp
+    -- simp
+    sorry
+
+/--
+Support of privMax_cut is bounded abouve by the cut number
+-/
+lemma privMax_cut_support_le_k (ε₁ ε₂ : ℕ+) (l : List ℕ) (N K : ℕ) (HKN : N ≤ K) :
+    privMax_cut ε₁ ε₂ l N K = 0 := by
+  induction N
+  · -- intro K HK HNK
+
+    induction K
+    · sorry
+    · sorry
+
+    -- simp_all only [CharP.cast_eq_zero]
+    -- rcases (lt_trichotomy K 0) with _ | ⟨H | _⟩ <;> try linarith
+    -- subst H
+    -- apply privMax_cut_boundary
+    -- simp
+  · rename_i n IH
+
+    -- -- intro K HK_nz HK_n'
+    -- unfold privMax_cut
+    -- simp
+    -- intro i
+    -- right
+    -- intro i'
+    -- right
+    -- intro a b HK
+    -- rw [probWhileCut_unfold_1]
+
+
+
+    sorry
+
+
+
 
 -- Since the max returnable value increases by at most 1 every iteration, and
 --    privMaxCut _ _ _ 0 = (fun _ => 0),
